updates

Veritas.MultiSet.fst
@@ -18,6 +18,10 @@ let lemma_eq_elim (#a:eqtype) (s1 s2: mset a):
   Lemma (requires (equal s1 s2))
         (ensures (s1 == s2)) = admit()
 
+let lemma_not_equal (#a:eqtype) (s1 s2: mset a) (x: a):
+  Lemma (requires (mem x s1 <> mem x s2))
+        (ensures (~(s1 == s2))) = admit()
+
 (* empty set *)
 let empty (#a:eqtype): Tot (mset a) = admit()
 
